Finish Lnodei

BPlusTree_Imp.thy
@@ -53,15 +53,17 @@ find_theorems list_assn
 find_theorems id_assn
 
 locale bplustree =
-  fixes A :: "'a \<Rightarrow> ('b::heap) \<Rightarrow> assn"
+  fixes A :: "'a \<Rightarrow> ('b::heap) \<Rightarrow> bool"
 begin
+
+definition "A_assn x y \<equiv> \<up>(A x y)"
 
 fun bplustree_assn :: "nat \<Rightarrow> 'a bplustree \<Rightarrow> 'b btnode ref \<Rightarrow> 'b btnode ref option \<Rightarrow> 'b btnode ref option \<Rightarrow> assn" where
   "bplustree_assn k (LNode xs) a r z = 
  (\<exists>\<^sub>A xsi xsi' fwd.
       a \<mapsto>\<^sub>r Btleaf xsi fwd
     * is_pfa (2*k) xsi' xsi
-    * list_assn A xs xsi'
+    * list_assn A_assn xs xsi'
     * \<up>(fwd = z)
     * \<up>(the r = a)
   )" |
@@ -72,7 +74,7 @@ fun bplustree_assn :: "nat \<Rightarrow> 'a bplustree \<Rightarrow> 'b btnode re
     * is_pfa (2*k) tsi' tsi
     * \<up>(length tsi' = length rs)
     * \<up>(tsi'' = zip (zip (map fst tsi') (zip (butlast (r#rs)) (butlast (rs@[z])))) (map snd tsi'))
-    * list_assn ((\<lambda> t (ti,r',z'). bplustree_assn k t (the ti) r' z') \<times>\<^sub>a A) ts tsi''
+    * list_assn ((\<lambda> t (ti,r',z'). bplustree_assn k t (the ti) r' z') \<times>\<^sub>a A_assn) ts tsi''
     )"
 
 find_theorems "map _ (zip _ _)"
@@ -89,7 +91,7 @@ fun btnode_assn :: "nat \<Rightarrow> 'a bplustree \<Rightarrow> 'b btnode \<Rig
   "btnode_assn k (LNode xs) (Btleaf xsi zi) r z = 
  (\<exists>\<^sub>A xsi xsi' zi.
     is_pfa (2*k) xsi' xsi
-    * list_assn A xs xsi'
+    * list_assn A_assn xs xsi'
     * \<up>(zi = z)
   )" |
   "btnode_assn k (Node ts t) (Btnode tsi ti) r z = 
@@ -98,11 +100,11 @@ fun btnode_assn :: "nat \<Rightarrow> 'a bplustree \<Rightarrow> 'b btnode \<Rig
     * is_pfa (2*k) tsi' tsi
     * \<up>(length tsi' = length rs)
     * \<up>(tsi'' = zip (zip (map fst tsi') (zip (butlast (r#rs)) (butlast (rs@[z])))) (map snd tsi'))
-    * list_assn ((\<lambda> t (ti,r',z'). bplustree_assn k t (the ti) r' z') \<times>\<^sub>a A) ts tsi''
+    * list_assn ((\<lambda> t (ti,r',z'). bplustree_assn k t (the ti) r' z') \<times>\<^sub>a A_assn) ts tsi''
     )" |
   "btnode_assn _ _ _ _ _ = false"
 
-abbreviation "blist_assn k ts tsi'' \<equiv> list_assn ((\<lambda> t (ti,r',z'). bplustree_assn k t (the ti) r' z') \<times>\<^sub>a A) ts tsi'' "
+abbreviation "blist_assn k ts tsi'' \<equiv> list_assn ((\<lambda> t (ti,r',z'). bplustree_assn k t (the ti) r' z') \<times>\<^sub>a A_assn) ts tsi'' "
 
 thm bplustree_assn.simps
 end
